src/simple-proof/Safety.v
@@ -27,6 +27,219 @@ Inductive normal_form: trm -> Prop :=
 
 Hint Constructors normal_form.
 
+(* Typing for the evaluation context / term pair with an empty typing context. Internally, a typing context representing the types of variables in the stack is used. *)
+Inductive ty_ec_trm: ctx -> ec -> trm -> typ -> Prop :=
+| ty_e_hole : forall G s t T,
+    G ~~ s ->
+    inert G ->
+    G |- t : T ->
+    ty_ec_trm G (e_hole s) t T
+| ty_e_term : forall L G s u t T U,
+    G ~~ s ->
+    inert G ->
+    G |- t : T ->
+    (forall x, x \notin L -> G & x ~ T |- (open_trm x u) : U) ->
+    ty_ec_trm G (e_term s u) t U.
+
+Lemma app_empty_inv: forall e s,
+    app_ec (e_hole empty) e (e_hole s) ->
+    e = e_hole s.
+Proof.
+  intros. inversions H. rewrite concat_empty_l. reflexivity.
+Qed.
+
+(* Lemma test_bnd: forall G x t T, *)
+(*     inert G -> *)
+(*     G |- trm_sel (avar_f x) t : T -> *)
+(*     exists T', G |- trm_var (avar_f x) : typ_bnd T'. *)
+(* Proof. *)
+(*   introv Hin Ht. apply (general_to_tight_typing Hin) in Ht. *)
+(*   inversions Ht. *)
+(*   - apply (invertible_typing_lemma Hin) in H3. *)
+(*     dependent induction H3. *)
+(*     + admit. *)
+(*     + eapply IHty_trm_inv; auto. *)
+(*   - admit. *)
+(* Qed. *)
+
+Lemma term_to_hole: forall s u t t',
+    red_ec (e_term s u) t (e_term s u) t' ->
+    red_ec (e_hole s) t (e_hole s) t'.
+Proof.
+  intros. dependent induction H.
+  - eapply red_ec_apply; eauto. 
+  - eapply red_ec_project; eauto.
+  - induction u; inversions x.
+    eapply IHu2; eauto.
+Qed.
+
+Lemma preservation_hole: forall G s t e' t' T,
+    red_ec (e_hole s) t e' t' ->
+    G ~~ s ->
+    inert G ->
+    G |- t : T ->
+    exists G', ty_ec_trm (G & G') e' t' T.
+Proof. 
+  introv Hred Hwf Hin Ht. 
+  dependent induction Ht; try solve [inversion Hred].
+  - admit.
+  - admit.
+  - inversions Hred.
+    exists (@empty typ). rewrite concat_empty_r.
+    eapply ty_e_term; eauto.
+  - specialize (IHHt Hred Hwf Hin) as [G' IHHt].
+    exists G'. inversions IHHt.
+    + eapply ty_e_hole; eauto.
+      apply weaken_subtyp with (G2:=G') in H; eauto.
+    + apply_fresh ty_e_term as z; eauto; intros. assert (z \notin L) by auto.
+      specialize (H3 z H4).
+      apply weaken_subtyp with (G2:=(G' & z ~ T0)) in H; rewrite concat_assoc in *; eauto.
+Qed.
+
+(* Lemma let_type: forall G t u T, *)
+(*     inert G -> *)
+(*     G |- trm_let t u : T -> *)
+(*     exists T', G |- t : T'. *)
+(* Proof. *)
+(*   introv Hin Ht. dependent induction Ht; eauto. *)
+(* Qed. *)
+
+(* Lemma let_open: forall L G t u T, *)
+(*     inert G -> *)
+(*     G |- trm_let t u : T -> *)
+(*     exists T', (forall x, x \notin L -> G & x ~ T' |- (open_trm x u) : T). *)
+(* Proof. *)
+(*   introv Hin Ht. dependent induction Ht; eauto. *)
+(* Qed. *)
+
+Lemma preservation'': forall G e t e' t' T,
+    red_ec e t e' t' ->
+    ty_ec_trm G e t T ->
+    exists G', ty_ec_trm (G & G') e' t' T.
+Proof.
+  introv Hred Ht.
+  inversions Ht.
+  { 
+    eapply preservation_hole; eauto.
+  }
+  {
+    rename H into Hwf. rename H0 into Hin.
+    rename H1 into Ht1. rename H2 into Ht2.
+    destruct t.
+    - inversions Hred.
+      pick_fresh y.
+      exists (@empty typ). rewrite concat_empty_r.
+      apply ty_e_hole; auto.
+      rewrite subst_intro_trm with (x:=y); auto.
+      rewrite <- subst_fresh_typ with (x:=y) (y:=x); auto.
+      eapply subst_ty_trm; eauto. rewrite~ subst_fresh_typ.
+    - inversions Hred.
+      pose proof (wf_sto_notin_dom Hwf H4).
+      pose proof (val_typing Ht1) as [V [Hv Hs]].
+      pick_fresh y. assert (y \notin L) by auto.
+      specialize (Ht2 y H0).
+      exists (x ~ V).
+      apply ty_e_hole.
+      * constructor~.
+        apply (precise_to_general Hv).
+      * constructor~.
+        apply (precise_inert_typ Hv).
+      * rewrite subst_intro_trm with (x:=y); auto.
+        rewrite <- subst_fresh_typ with (x:=y) (y:=x); auto.
+        eapply subst_ty_trm; eauto.
+        { eapply weaken_rules; eauto. }
+        { apply~ fv_ctx_types_push. }
+        {
+          rewrite~ subst_fresh_typ.
+          pose proof (ty_var (binds_tail x V G)).
+          apply (ty_sub H1). apply (weaken_subtyp Hs); eauto.
+        }
+    - inversion Hred. rewrite <- H3 in Hred. apply term_to_hole in Hred. subst.
+      pose proof (preservation_hole Hred Hwf Hin Ht1) as [G' Ht].
+      inversions Ht.
+      exists G'.
+      eapply ty_e_term with (L:=L \u (dom G) \u (dom G')); eauto. intros. 
+      assert (x0 \notin L) by auto.
+      specialize (Ht2 x0 H3).
+      eapply (proj41 weaken_rules); eauto.
+    - inversion Hred. rewrite <- H1 in Hred. apply term_to_hole in Hred. subst.
+      pose proof (preservation_hole Hred Hwf Hin Ht1) as [G' Ht].
+      inversions Ht.
+      exists G'.
+      eapply ty_e_term with (L:=L \u (dom G) \u (dom G')); eauto. intros. 
+      assert (x0 \notin L) by auto.
+      specialize (Ht2 x0 H2).
+      eapply (proj41 weaken_rules); eauto.
+    - (* lemma for type of t1 *)
+      inversions Hred.
+      (* rename t' into t1. rename u into t3. *)
+      (* rename T into T3. rename T0 into T2. *)
+      (* pose proof (let_type Hin Ht1) as [T1 Ht']. *)
+      exists (@empty typ). rewrite concat_empty_r.
+      gen L.
+      dependent induction Ht1; intros.
+      + eapply ty_e_term with (L:=L); eauto. intros.
+        unfold open_trm. simpl. specialize (H x H1).
+        apply_fresh ty_let as z; eauto. admit.
+      + eapply IHHt1 with (L:=L \u (dom G)); eauto. intros. 
+        assert (x \notin L) by auto.
+        specialize (Ht2 x H1).
+        eapply narrow_typing; eauto. apply~ subenv_last.
+  }
+Qed.
+
+Lemma open_1_test: forall G t y n T,
+    G |- t : T ->
+    n > 0 ->
+    t = (open_rec_trm n y t).
+    (* G & x ~ U |- open_trm x (open_rec_trm 1 y u) : T. *)
+Proof.
+  intros. gen G T y. induction t; intros.
+  - destruct a.
+    + simpl. case_if~. subst.
+      apply var_typing_implies_avar_f in H. destruct H. inversion H.
+    + reflexivity.
+  - destruct v. 
+    + simpl. dependent induction H; eauto. admit.
+    + simpl. dependent induction H; eauto. admit.
+  - destruct a. 
+    + simpl. case_if~. subst. dependent induction H; eauto. 
+    + reflexivity.
+  - destruct a; destruct a0.
+    + simpl. 
+      repeat case_if; subst; dependent induction H; eauto; case_if. 
+    + simpl. case_if; subst; dependent induction H; eauto; case_if. 
+    + simpl. case_if; subst; dependent induction H; eauto; case_if. 
+    + reflexivity.
+  - simpl. dependent induction H; eauto.
+    replace (trm_let t1 t2) with (trm_let (open_rec_trm 1 y t1) t2).
+    + simpl. admit.
+    + specialize (IHt1 _ _ H y). rewrite <- IHt1. reflexivity.
+Qed.
+
+(* Lemma preservation': forall G e t e' t' T, *)
+(*     G ~~ (ec_sto e) -> *)
+(*     inert G -> *)
+(*     red_ec e t e' t' -> *)
+(*     G |- t : T -> *)
+(*     exists G', inert G' /\ *)
+(*           G & G' ~~ (ec_sto e') /\ *)
+(*           G & G' |- t' : T. *)
+(* Proof. *)
+(*   introv Hwf Hin Hred Ht. gen t'. *)
+(*   dependent induction Ht; intros. *)
+(*   - dependent induction Hred. *)
+(*     +  *)
+(*     + inversions Hred. admit. *)
+(*     + dependent induction Hred. *)
+(*       * admit. *)
+(*       *  *)
+(*   (* - admit. *) *)
+(*   (* - admit.  *) *)
+(*   (* - inversions Hred. *) *)
+(* Admitted. *)
+            
+
 Lemma preservation: forall G s t s' t' T,
     G ~~ s ->
     inert G ->
@@ -99,6 +312,181 @@ Proof.
     apply weaken_subtyp with (G2:=G') in H.
     + apply (ty_sub Ht' H).
     + eauto.
+Qed.
+
+Lemma app_hole_empty_hole: forall s,
+    app_ec (e_hole s) (e_hole empty) (e_hole s).
+Proof.
+  intros. replace (app_ec (e_hole s) (e_hole empty) (e_hole s)) with (app_ec (e_hole s) (e_hole empty) (e_hole (s & empty))).
+  - apply app_hole_hole. admit.
+  - rewrite concat_empty_r. reflexivity.
+Qed.
+
+Lemma app_hole_empty_term: forall s t,
+    app_ec (e_hole s) (e_term empty t) (e_term s t).
+Proof.
+  intros. 
+  replace (e_term s t) with (e_term (s & empty) t).
+  - apply app_hole_term. admit.
+  - rewrite concat_empty_r. reflexivity.
+Qed.
+
+Lemma progress'': forall G e t T,
+    ty_ec_trm G e t T ->
+    (normal_form t \/ exists e' t', red_ec e t e' t').
+Proof.
+  intros. destruct e.
+  {
+    inversions H. rename H1 into Hwf. rename H2 into Hin. rename H4 into Ht.
+    dependent induction Ht; try solve [left; auto].
+    - admit.
+    - admit.
+    - right. exists (e_term s u) t.
+      apply red_ec_hole_to_term.
+      (* destruct t. *)
+      (* + pose proof (var_typing_implies_avar_f Ht) as [x A]. subst. *)
+      (*   exists (e_term s u) (trm_var (avar_f x)). *)
+      (*   apply red_ec_hole_to_term. *)
+      (* + pick_fresh x. *)
+      (*   exists (e_term s u) (trm_val v). *)
+      (*   apply red_ec_hole_to_term. *)
+      (* + specialize (IHHt Hwf Hin) as [IH | [e' [t' Hred]]]. *)
+      (*   * inversion IH. *)
+      (*   * exists (e_term s u) (trm_sel a t). *)
+      (*     apply red_ec_hole_to_term.  *)
+      (* + specialize (IHHt Hwf Hin) as [IH | [e' [t' Hred]]]. *)
+      (*   * inversion IH. *)
+      (*   * exists (e_term s u) (trm_app a a0). *)
+      (*     apply red_ec_hole_to_term.  *)
+      (* + specialize (IHHt Hwf Hin) as [IH | [e' [t' Hred]]]. *)
+      (*   * inversion IH. *)
+      (*   * exists (e_term s u) (trm_let t1 t2). *)
+      (*     apply red_ec_hole_to_term.  *)
+    - specialize (IHHt Hwf Hin) as [IH | [t' [s' Hred]]].
+      + left. assumption.
+      + right. exists t' s'. assumption.
+  }
+  {
+    inversions H. 
+    rename H2 into Hwf. rename H3 into Hin. rename H5 into Ht. clear H8.
+    dependent induction Ht; try solve [left; auto].
+    - right. admit.
+    - right. admit.
+    - right. exists (e_term s (trm_let u t0)) t.
+      eapply red_ec_let_let.
+      (* destruct t. *)
+      (* + pose proof (var_typing_implies_avar_f Ht) as [x A]. subst. *)
+      (*   pose proof (app_hole_empty_term s t0). *)
+      (*   pose proof (app_hole_empty_term s (trm_let u t0)). *)
+      (*   exists (e_term s (trm_let u t0)) (trm_var (avar_f x)). *)
+      (*   eapply (red_ec_term (red_ec_let_let (trm_var (avar_f x)) u t0) H1 H2). *)
+      (* + pick_fresh x. *)
+      (*   pose proof (app_hole_empty_term s t0). *)
+      (*   pose proof (app_hole_empty_term s (trm_let u t0)). *)
+      (*   exists (e_term s (trm_let u t0)) (trm_val v). *)
+      (*   eapply (red_ec_term (red_ec_let_let (trm_val v) u t0) H1 H2). *)
+      (* + specialize (IHHt Hwf Hin) as [IH | [e' [t' Hred]]]. *)
+      (*   * inversion IH. *)
+      (*   * exists (e_term s (trm_let u t0)) (trm_sel a t). *)
+      (*     pose proof (app_hole_empty_term s t0). *)
+      (*     pose proof (app_hole_empty_term s (trm_let u t0)). *)
+      (*     apply (red_ec_term (red_ec_let_let (trm_sel a t) u t0) H1 H2). *)
+      (* + specialize (IHHt Hwf Hin) as [IH | [e' [t' Hred]]]. *)
+      (*   * inversion IH. *)
+      (*   * exists (e_term s (trm_let u t0)) (trm_app a a0). *)
+      (*     pose proof (app_hole_empty_term s t0). *)
+      (*     pose proof (app_hole_empty_term s (trm_let u t0)). *)
+      (*     eapply (red_ec_term (red_ec_let_let (trm_app a a0) u t0) H1 H2). *)
+      (* + specialize (IHHt Hwf Hin) as [IH | [e' [t' Hred]]]. *)
+      (*   * inversion IH. *)
+      (*   * exists (e_term s (trm_let u t0)) (trm_let t1 t2). *)
+      (*     pose proof (app_hole_empty_term s t0). *)
+      (*     pose proof (app_hole_empty_term s (trm_let u t0)). *)
+      (*     eapply (red_ec_term (red_ec_let_let (trm_let t1 t2) u t0) H1 H2). *)
+    - specialize (IHHt Hwf Hin) as [IH | [t' [s' Hred]]].
+      + left. assumption.
+      + right. exists t' s'. assumption.
+  }
+Qed.
+
+
+Lemma progress': forall G t e T,
+    G ~~ (ec_sto e) ->
+    inert G ->
+    G |- t : T ->
+    (normal_form t \/ exists e' t', red_ec e t e' t').
+Proof.
+  introv Hwf Hin Ht. dependent induction Ht; try solve [left; auto].
+  - right. admit.
+  - right. admit.
+  - right. destruct t.
+    + pose proof (var_typing_implies_avar_f Ht) as [x A]. subst.
+      destruct e.
+      {
+        exists (e_term s u) (trm_var (avar_f x)).
+        apply red_ec_hole_to_term.
+      }
+      {
+        pose proof (app_hole_empty_term s t).
+        pose proof (app_hole_empty_term s (trm_let u t)).
+        exists (e_term s (trm_let u t)) (trm_var (avar_f x)).
+        eapply (red_ec_term (red_ec_let_let (trm_var (avar_f x)) u t) H1 H2).
+      } 
+    + pick_fresh x.
+      destruct e.
+      {
+        exists (e_term s u) (trm_val v).
+        apply red_ec_hole_to_term.
+      }
+      {
+        pose proof (app_hole_empty_term s t).
+        pose proof (app_hole_empty_term s (trm_let u t)).
+        exists (e_term s (trm_let u t)) (trm_val v).
+        eapply (red_ec_term (red_ec_let_let (trm_val v) u t) H1 H2).
+      }
+    + specialize (IHHt Hwf Hin) as [IH | [e' [t' Hred]]].
+      * inversion IH.
+      * destruct e.
+        { 
+          exists (e_term s u) (trm_sel a t).
+          apply red_ec_hole_to_term. 
+        }
+        {
+          exists (e_term s (trm_let u t0)) (trm_sel a t).
+          (* TODO: change to lemma *)
+          pose proof (app_hole_empty_term s t0).
+          pose proof (app_hole_empty_term s (trm_let u t0)).
+          apply (red_ec_term (red_ec_let_let (trm_sel a t) u t0) H1 H2).
+        } 
+    + specialize (IHHt Hwf Hin) as [IH | [e' [t' Hred]]].
+      * inversion IH.
+      * destruct e.
+        { 
+          exists (e_term s u) (trm_app a a0).
+          apply red_ec_hole_to_term. 
+        }
+        {
+          exists (e_term s (trm_let u t)) (trm_app a a0).
+          pose proof (app_hole_empty_term s t).
+          pose proof (app_hole_empty_term s (trm_let u t)).
+          eapply (red_ec_term (red_ec_let_let (trm_app a a0) u t) H1 H2).
+        } 
+    + specialize (IHHt Hwf Hin) as [IH | [e' [t' Hred]]].
+      * inversion IH.
+      * destruct e.
+        {
+          exists (e_term s u) (trm_let t1 t2).
+          apply red_ec_hole_to_term. 
+        }
+        {
+          exists (e_term s (trm_let u t)) (trm_let t1 t2).
+          pose proof (app_hole_empty_term s t).
+          pose proof (app_hole_empty_term s (trm_let u t)).
+          eapply (red_ec_term (red_ec_let_let (trm_let t1 t2) u t) H1 H2).
+        } 
+  - specialize (IHHt Hwf Hin) as [IH | [t' [s' Hred]]].
+    + left. assumption.
+    + right. exists t' s'. assumption.
 Qed.
 
 Lemma progress: forall G t s T,
