src/simple-proof/Some_lemmas.v
@@ -194,24 +194,24 @@ Proof.
     subst~.
 Qed.
 
-Lemma open_fresh_ec_injective : forall e e' z,
-    z \notin fv_ec e ->
-    z \notin fv_ec e' ->
-    open_ec z e = open_ec z e' ->
-    e = e'.
-Proof.
-  intros. dependent induction e; destruct e'; inversions H1.
-  - reflexivity.
-  - simpl in *. 
-    apply (proj42 open_fresh_trm_val_def_defs_injective) in H4; auto.
-    assert (e = e'). {
-      eapply IHe; auto.
-    }
-    subst. reflexivity.
-  - simpl in *.
-    apply (proj41 open_fresh_trm_val_def_defs_injective) in H4; auto.
-    subst. reflexivity.
-Qed.
+(* Lemma open_fresh_ec_injective : forall e e' z, *)
+(*     z \notin fv_ec e -> *)
+(*     z \notin fv_ec e' -> *)
+(*     open_ec z e = open_ec z e' -> *)
+(*     e = e'. *)
+(* Proof. *)
+(*   intros. dependent induction e; destruct e'; inversions H1. *)
+(*   - reflexivity. *)
+(*   - simpl in *.  *)
+(*     apply (proj42 open_fresh_trm_val_def_defs_injective) in H4; auto. *)
+(*     assert (e = e'). { *)
+(*       eapply IHe; auto. *)
+(*     } *)
+(*     subst. reflexivity. *)
+(*   - simpl in *. *)
+(*     apply (proj41 open_fresh_trm_val_def_defs_injective) in H4; auto. *)
+(*     subst. reflexivity. *)
+(* Qed. *)
 
 (* ###################################################################### *)
 
